@prefix schema: <http://schema.org/> .
@prefix rdfs: <http://www.w3.org/2000/01/rdf-schema#> .
@prefix dc: <http://purl.org/dc/terms/> .
@prefix rdf: <http://www.w3.org/1999/02/22-rdf-syntax-ns#> .

schema:LabProtocol
  a rdfs:Class ;
  schema:isPartOf <http://bio.schema.org> ;
  rdfs:label "LabProtocol" ;
  rdfs:comment "An experimental protocol is a sequence of tasks and operations executed to perform experimental research in biological and biomedical areas." ;
  rdfs:subClassOf schema:CreativeWork ;
  dc:source <http://bioschemas.org> .





schema:bioSampleUsed
  a rdf:Property ;
  schema:isPartOf <http://bio.schema.org> ;
  rdfs:label "bioSampleUsed" ;
  rdfs:comment "BioSample used in the protocol. It could be a record in a Dataset describing the sample or a physical object corresponding to the sample or a URL pointing to the type of sample used." ;
  schema:domainIncludes schema:LabProtocol ;
  schema:rangeIncludes schema:BioChemEntity, schema:BioSample, schema:DefinedTerm, schema:Text, schema:URL, schema:Taxon, ;
  dc:source <http://www.bioschemas.org/LabProtocol> .

schema:labEquipmentUsed
  a rdf:Property ;
  schema:isPartOf <http://bio.schema.org> ;
  rdfs:label "labEquipmentUsed" ;
  rdfs:comment "A laboratory equipment used by a person to follow one or more steps described in this LabProtocol." ;
  schema:domainIncludes schema:LabProtocol ;
  schema:rangeIncludes schema:DefinedTerm, schema:Text, schema:URL ;
  dc:source <http://www.bioschemas.org/LabProtocol> .

schema:protocolPurpose
  a rdf:Property ;
  schema:isPartOf <http://bio.schema.org> ;
  rdfs:label "protocolPurpose" ;
  rdfs:comment "The purpose of the protocol enables readers to make a decision as to the suitability of the protocol to their experimental problem. (see more information at http://vocab.linkeddata.es/SMARTProtocols/myDocumentation_SPdoc_18Abril2017/index_SPdoc_V4.0.html#PurposeOfProtocol)." ;
  schema:domainIncludes schema:LabProtocol ;
  schema:rangeIncludes schema:CreativeWork, schema:Text ;
  dc:source <http://www.bioschemas.org/LabProtocol> .

schema:reagentUsed
  a rdf:Property ;
  schema:isPartOf <http://bio.schema.org> ;
  rdfs:label "reagentUsed" ;
  rdfs:comment "Reagents used in the protocol. ChEBI and PubChem entities can be used whenever available. Commercial names are also acceptable (URL if possible)." ;
  schema:domainIncludes schema:LabProtocol ;
  schema:rangeIncludes schema:BioChemEntity, schema:DefinedTerm, schema:Text, schema:URL ;
  dc:source <http://www.bioschemas.org/LabProtocol> .  



     

schema:protocolAdvantage
  a rdf:Property ;
  schema:isPartOf <http://bio.schema.org> ;
  rdfs:label "protocolAdvantage" ;
  rdfs:comment "Situations where the Protocol has been successfully employed (see more information at http://vocab.linkeddata.es/SMARTProtocols/myDocumentation_SPdoc_18Abril2017/index_SPdoc_V4.0.html#AdvantageOfTheProtocol)" ;
  schema:domainIncludes schema:LabProtocol ;
  schema:rangeIncludes schema:CreativeWork, schema:Text ;
  dc:source <http://www.bioschemas.org/LabProtocol> .

schema:protocolApplication
  a rdf:Property ;
  schema:isPartOf <http://bio.schema.org> ;
  rdfs:label "protocolApplication" ;
  rdfs:comment "Applications of the protocol list the full diversity of the applications of the method and support if is possible to extend the range of applications of the protocol. e.g. northern blot assays, sequencing, etc. (see more information at http://vocab.linkeddata.es/SMARTProtocols/myDocumentation_SPdoc_18Abril2017/index_SPdoc_V4.0.html#ApplicationOfTheProtocol)" ;
  schema:domainIncludes schema:LabProtocol ;
  schema:rangeIncludes schema:CreativeWork, schema:Text ;
  dc:source <http://www.bioschemas.org/LabProtocol> .  

schema:protocolLimitation
  a rdf:Property ;
  schema:isPartOf <http://bio.schema.org> ;
  rdfs:label "protocolLimitation" ;
  rdfs:comment "Situations where the Protocol would be unreliable or otherwise unsuccessful (see more information at http://vocab.linkeddata.es/SMARTProtocols/myDocumentation_SPdoc_18Abril2017/index_SPdoc_V4.0.html#LimitationOfTheProtocol)" ;
  schema:domainIncludes schema:LabProtocol ;
  schema:rangeIncludes schema:CreativeWork, schema:Text ;
  dc:source <http://www.bioschemas.org/LabProtocol> .  

schema:protocolOutcome
  a rdf:Property ;
  schema:isPartOf <http://bio.schema.org> ;
  rdfs:label "protocolOutcome" ;
  rdfs:comment "Outcome or expected result by a protocol execution (see more information at http://vocab.linkeddata.es/SMARTProtocols/myDocumentation_SPdoc_18Abril2017/index_SPdoc_V4.0.html#OutcomeOfTheProtocol)" ;
  schema:domainIncludes schema:LabProtocol ;
  schema:rangeIncludes schema:CreativeWork, schema:Text ;
  dc:source <http://www.bioschemas.org/LabProtocol> .  

schema:softwareUsed
  a rdf:Property ;
  schema:isPartOf <http://bio.schema.org> ;
  rdfs:label "softwareUsed" ;
  rdfs:comment "Software or tool used as part of the lab protocol to complete a part of it." ;
  schema:domainIncludes schema:LabProtocol ;
  schema:rangeIncludes schema:SoftwareApplication, schema:URL ;
  dc:source <http://www.bioschemas.org/LabProtocol> .  


schema:totalTime
  a rdf:Property ;
  rdfs:label "totalTime" ;
  rdfs:comment "The total time required to perform instructions or a direction (including time to prepare the supplies), in ISO 8601 duration format." ;
  schema:domainIncludes schema:LabProtocol ;
  schema:rangeIncludes schema:Duration . 






